Developed a new CSR interface in which each CSR field has an associated predicate and an associated transformation funtion. Whenever the processor attempts to write to a CSR field, it checks whether or not the given value satisfies the field predicate. If so, it writes the value. Otherwise, it applies the transformation function and writes the result. Ive ported the existing CSR database to use the new CSR interface and commented out the old code.

FU.v
@@ -235,12 +235,16 @@ Section Params.
                                  "reg_data" :: Maybe Data }.
 
   Definition IntRegWrite := STRUCT {
-                             "addr" :: RegId ;
-                             "data" :: Array 1 (Bit Xlen) }.
+                             "index" :: RegId ;
+                             "data" :: Bit Xlen }.
 
   Definition FloatRegWrite := STRUCT {
-                               "addr" :: RegId ;
-                               "data" :: Array 1 (Bit Flen) }.
+                               "index" :: RegId ;
+                               "data" :: Bit Flen }.
+
+  Definition CsrWrite := STRUCT {
+                             "addr" :: CsrId ;
+                             "data" :: CsrValue }.
 
   Definition MemWrite := STRUCT {
                              "addr" :: VAddr ;
@@ -259,11 +263,10 @@ Section Params.
                                }.
 
   Definition CSRWriteState
-    (k : Kind)
     :  Kind
     := STRUCT {
-         "csrValueCurrent" :: k;
-         "csrValueToWrite" :: k;
+         (* "csrValueCurrent" :: k; *)
+         (* "csrValueToWrite" :: k; *)
          "pc" :: VAddr;
          "compressed?" :: Bool
        }.
@@ -412,6 +415,7 @@ Section Params.
     Local Notation LocationReadWriteInputT := (LocationReadWriteInputT 0 CsrIdWidth 2).
     
     (* Represents CSR entry fields. *)
+(*
     Local Definition csrField (k : Kind) (value : option (ConstT k))
       :  {k : Kind & option (ConstT k)}
       := existT (fun k => option (ConstT k)) k value.
@@ -430,6 +434,828 @@ Section Params.
                   view_kind    := x
                 |} :: repeatView k x)%vector
            end.
+
+    Definition MayStructField
+      :  Type
+      := string * {k : Kind & option (ConstT k)}.
+*)
+    Record CSRField
+      := {
+           csrFieldName : string;
+           csrFieldKind : Kind;
+           csrFieldDefaultValue : option (ConstT csrFieldKind);
+           csrFieldIsValid
+             : ContextCfgPkt @# ty ->
+               CSRWriteState @# ty ->
+               csrFieldKind @# ty ->
+               csrFieldKind @# ty ->
+               Bool @# ty;
+           csrFieldXform
+             : ContextCfgPkt @# ty ->
+               CSRWriteState @# ty ->
+               csrFieldKind @# ty ->
+               csrFieldKind @# ty ->
+               csrFieldKind @# ty
+         }.
+
+    Record CSRView
+      := {
+           csrViewContext : Bit 2 @# ty;
+           csrViewNumFields : nat;
+           csrViewFields : Vector.t CSRField csrViewNumFields
+         }.
+
+    Record CSR :=
+      {
+        csrName : string;
+        csrAddr : word CsrIdWidth;
+        csrViews : Vector.t CSRView 2
+      }.
+
+    Definition csrViewKind
+      (view : CSRView)
+      :  Kind
+      := Struct
+           (Vector.nth
+             (Vector.map
+               csrFieldKind
+               (csrViewFields view)))
+           (Vector.nth
+             (Vector.map
+               csrFieldName
+               (csrViewFields view))).
+
+    Definition csrViewMayStruct
+      (view : CSRView)
+      :  MayStruct (csrViewNumFields view)
+      := Build_MayStruct
+           (Vector.nth 
+             (Vector.map
+               (fun field
+                 => existT
+                      (fun k => option (ConstT k))
+                      (csrFieldKind field)
+                      (csrFieldDefaultValue field))
+               (csrViewFields view)))
+           (Vector.nth 
+             (Vector.map
+               csrFieldName
+               (csrViewFields view))).
+
+    Open Scope kami_action.
+
+    (* TODO: replace with pre-existing theorem in VectorDef. *)
+    Theorem nth_map
+      : forall (A B : Type)
+          (f : A -> B)
+          (n : nat)
+          (i : Fin.t n)
+          (xs : Vector.t A n),
+          f (Vector.nth xs i) = Vector.nth (Vector.map f xs) i.
+    Proof
+      fun A B f
+        => Fin.t_ind
+             (fun (n : nat) (i : Fin.t n)
+               => forall xs : Vector.t A n,
+                    f (Vector.nth xs i) = Vector.nth (Vector.map f xs) i)
+             (fun (n : nat) (xs : Vector.t A (S n))
+               => caseS
+                    (fun (n : nat) (xs : Vector.t A (S n))
+                      => f (Vector.nth xs Fin.F1) = Vector.nth (Vector.map f xs) Fin.F1)
+                    (fun (x0 : A) (n : nat) (_ : Vector.t A n)
+                      => eq_refl (f x0))
+                    xs)
+             (fun (n : nat) (i : Fin.t n)
+               (H : forall xs : Vector.t A n,
+                      f (Vector.nth xs i) = Vector.nth (Vector.map f xs) i)
+               (xs : Vector.t A (S n))
+               => caseS
+                    (fun (m : nat) (ys : Vector.t A (S m))
+                      => forall
+                           (j : Fin.t m)
+                           (H0 : forall ys : Vector.t A m,
+                                   f (Vector.nth ys j) = Vector.nth (Vector.map f ys) j),
+                           f (Vector.nth ys (Fin.FS j)) = Vector.nth (Vector.map f ys) (Fin.FS j))
+                    (fun (y0 : A) (m : nat) (ys : Vector.t A m)
+                      (j : Fin.t m)
+                      (H0 : _)
+                      => H0 ys)
+                    xs i H).
+
+    Lemma gen_nth_map
+      : forall (A B : Type)
+          (f : A -> B)
+          (n : nat)
+          (xs : Vector.t A n),
+          (fun i => f (Vector.nth xs i)) = Vector.nth (Vector.map f xs).
+    Proof
+      fun (A B : Type) (f : A -> B) (n : nat) (xs : t A n)
+        => functional_extensionality
+             (fun i : Fin.t n => f xs[@i])
+             (Vector.nth (Vector.map f xs))
+             (fun i : Fin.t n => nth_map f i xs).
+
+(*
+Coq < Show Script.
+Proof.
+intro.
+(unfold csrViewKind).
+(apply (f_equal2 (@Struct (csrViewNumFields view)))).
+ (rewrite
+   <- (gen_nth_map
+         (fun field : CSRField =>
+          existT (fun k => option (ConstT k)) (csrFieldKind field)
+            (csrFieldDefaultValue field)) (csrViewFields view))).
+ (simpl).
+ symmetry.
+ (apply gen_nth_map).
+
+ reflexivity.
+
+Qed.
+*)
+    Lemma csrViewKindCorrect
+      : forall view : CSRView,
+          csrViewKind view =
+          Struct
+             (fun i : Fin.t (csrViewNumFields view)
+               => projT1
+                    (Vector.nth
+                      (Vector.map
+                        (fun field : CSRField
+                          => existT
+                               (fun k : Kind => option (ConstT k))
+                               (csrFieldKind field)
+                               (csrFieldDefaultValue field))
+                        (csrViewFields view))
+                      i))
+           (Vector.nth
+             (Vector.map
+               csrFieldName
+               (csrViewFields view))).
+      Proof
+        fun view
+          => f_equal2
+               (@Struct (csrViewNumFields view))
+               (eq_ind
+                 (fun i
+                   => existT
+                        (fun k => option (ConstT k))
+                        (csrFieldKind (Vector.nth (csrViewFields view) i))
+                        (csrFieldDefaultValue (Vector.nth (csrViewFields view) i)))
+                 (fun s
+                   => Vector.nth
+                        (Vector.map csrFieldKind (csrViewFields view)) =
+                      (fun i => projT1 (s i)))
+                 (eq_sym (gen_nth_map csrFieldKind (csrViewFields view)))
+                 (Vector.nth
+                   (Vector.map
+                     (fun field
+                       => existT
+                            (fun k => option (ConstT k))
+                            (csrFieldKind field)
+                            (csrFieldDefaultValue field))
+                     (csrViewFields view)))
+                 (gen_nth_map
+                   (fun field
+                     => existT
+                          (fun k => option (ConstT k))
+                          (csrFieldKind field)
+                          (csrFieldDefaultValue field))
+                   (csrViewFields view)))
+               eq_refl.
+
+    Definition csrViewReadWrite
+      (view : CSRView)
+      (k : Kind)
+      (cfg_pkt : ContextCfgPkt @# ty)
+      (context_pkt : CSRWriteState @# ty)
+      (req : LocationReadWriteInputT k @# ty)
+      :  ActionT ty k
+      := LETA csr_value
+           :  csrViewKind view
+           <- eq_rect_r
+                (ActionT ty)
+                (MayStruct_RegReads ty (csrViewMayStruct view))
+                (csrViewKindCorrect view);
+         If !(req @% "isRd")
+           then
+             LET input_value
+               :  csrViewKind view
+               <- unpack
+                    (csrViewKind view)
+                    (ZeroExtendTruncLsb
+                      (size (csrViewKind view))
+                      (pack (req @% "data")));
+             LET write_value
+               :  csrViewKind view
+               <- BuildStruct 
+                    (Vector.nth
+                      (Vector.map
+                        csrFieldKind
+                        (csrViewFields view)))
+                    (Vector.nth
+                      (Vector.map
+                        csrFieldName
+                        (csrViewFields view)))
+                    (fun i : Fin.t (csrViewNumFields view)
+                      => let field
+                           :  CSRField 
+                           := Vector.nth (csrViewFields view) i in
+                         let field_kind
+                           :  Kind
+                           := csrFieldKind field in
+                         let curr_field_value
+                           :  field_kind @# ty
+                           := eq_rect_r
+                                (fun t => Expr ty (SyntaxKind t))
+                                (ReadStruct #csr_value i)
+                                (nth_map csrFieldKind i (csrViewFields view))
+                         in
+                         let input_field_value
+                           :  field_kind @# ty
+                           := eq_rect_r 
+                                (fun t => Expr ty (SyntaxKind t))
+                                (ReadStruct #input_value i)
+                                (nth_map csrFieldKind i (csrViewFields view))
+                         in
+                         eq_rect
+                           field_kind
+                           (fun t => Expr ty (SyntaxKind t))
+                           (ITE
+                             (csrFieldIsValid field
+                               cfg_pkt
+                               context_pkt
+                               curr_field_value
+                               input_field_value)
+                             input_field_value
+                             (csrFieldXform field
+                               cfg_pkt
+                               context_pkt
+                               curr_field_value
+                               input_field_value))
+                           (Vector.nth (Vector.map csrFieldKind (csrViewFields view)) i)
+                           (nth_map csrFieldKind i (csrViewFields view)));
+             LETA _
+               : Void 
+               <- MayStruct_RegWrites (csrViewMayStruct view)
+                    (eq_rect
+                      (csrViewKind view)
+                      (fun t => Expr ty (SyntaxKind t))
+                      #write_value
+                      (Struct
+                        (fun i => projT1 (vals (csrViewMayStruct view) i))
+                        (names (csrViewMayStruct view)))
+                      (csrViewKindCorrect view));
+             Retv;
+         Ret
+           (unpack k
+             (ZeroExtendTruncLsb (size k)
+               (pack (#csr_value)))).
+
+    Definition csrReadWrite
+      (entries : list CSR)
+      (k : Kind)
+      (cfg_pkt : ContextCfgPkt @# ty)
+      (context_pkt : CSRWriteState @# ty)
+      (req : LocationReadWriteInputT k @# ty)
+      :  ActionT ty (Maybe k)
+      := System [
+           DispString _ "[csrReadWrite]\n";
+           DispString _ "[csrReadWrite] request:\n";
+           DispHex req;
+           DispString _ "\n"
+         ];
+         utila_acts_find_pkt
+           (map
+             (fun csr_entry : CSR
+               => utila_acts_find_pkt
+                    (map
+                      (fun view_entry : CSRView
+                        => LET entry_match
+                             :  Bool
+                             <- ((req @% "addr") == $$(csrAddr csr_entry) &&
+                                 (req @% "contextCode") == csrViewContext view_entry);
+                           If #entry_match
+                             then
+                               System [
+                                 DispString _ "[csrReadWrite]\n";
+                                 DispString _ "  csr name: ";
+                                 DispString _ (csrName csr_entry);
+                                 DispString _ "\n"
+                               ];
+                               csrViewReadWrite view_entry cfg_pkt context_pkt req 
+                             else
+                               Ret (unpack k $0)
+                             as result;
+                           (utila_acts_opt_pkt #result #entry_match))
+                      (Vector.to_list
+                        (csrViews csr_entry))))
+             entries).
+
+    Definition csrFieldReserved
+      (name : string)
+      (n : nat)
+      :  CSRField
+      := {|
+           csrFieldName := name;
+           csrFieldKind := Bit n;
+           csrFieldDefaultValue := Some (ConstBit (natToWord n 0));
+           csrFieldIsValid
+             := fun _ _ _ _ => $$false;
+           csrFieldXform
+             := fun _ _ _ _ => Const ty (natToWord n 0);
+         |}.
+
+    Definition csrFieldAny
+      (name : string)
+      (n : nat)
+      (default : option (ConstT (Bit n)))
+      :  CSRField
+      := {| 
+           csrFieldName := ^name;
+           csrFieldKind := Bit n;
+           csrFieldDefaultValue := default;
+           csrFieldIsValid
+             := fun _ _ _ _ => $$true;
+           csrFieldXform
+             := fun _ _ _ => id
+         |}.
+
+    Fixpoint repeatCSRView
+      (n m : nat)
+      (fields : Vector.t CSRField m)
+      :  Vector.t CSRView n
+      := match n with
+           | 0 => []%vector
+           | S k
+             => ({|
+                   csrViewContext   := $n;
+                   csrViewNumFields := m;
+                   csrViewFields    := fields
+                 |} :: repeatCSRView k fields)%vector
+           end.
+
+    Definition xlField
+      (prefix : string)
+      :  CSRField
+      := {|
+           csrFieldName := ^(prefix ++ "xl");
+           csrFieldKind := Bit 2;
+           csrFieldDefaultValue := None; (* TODO *)
+           csrFieldIsValid
+             := fun _ _ _ x
+                  => x == $1 || x == $2;
+           csrFieldXform
+             := fun _ _ curr_value _
+                  => curr_value
+         |}.
+
+    Definition CSRs
+      :  list CSR
+      := [
+           {|
+             csrName := ^"fflagsG";
+             csrAddr := natToWord CsrIdWidth 1;
+             csrViews
+               := repeatCSRView 2
+                    [
+                      csrFieldReserved "reserved" 27;
+                      @csrFieldAny "fflags" 5 None
+                    ]%vector
+           |};
+           {|
+             csrName := ^"frmG";
+             csrAddr := natToWord CsrIdWidth 2;
+             csrViews
+               := repeatCSRView 2
+                    [
+                      csrFieldReserved "reserved" 29;
+                      @csrFieldAny "frm" 3 None
+                    ]%vector
+           |};
+           {|
+             csrName := ^"fstatusG";
+             csrAddr := natToWord CsrIdWidth 3;
+             csrViews
+               := repeatCSRView 2
+                    [
+                      csrFieldReserved "reserved" 24;
+                      @csrFieldAny "frm" 3 None;
+                      @csrFieldAny "fflags" 5 None
+                    ]%vector
+           |};
+           {|
+             csrName := ^"misa";
+             csrAddr := CsrIdWidth 'h"301";
+             csrViews
+               := [
+                    {|
+                      csrViewContext := $1;
+                      csrViewNumFields := 3;
+                      csrViewFields
+                        := [
+                             xlField "m";
+                             csrFieldReserved "reserved" 4;
+                             @csrFieldAny "extensions" 26 None (* TODO *)
+                           ]%vector
+                    |};
+                    {|
+                      csrViewContext := $2;
+                      csrViewNumFields := 3;
+                      csrViewFields
+                        := [
+                             xlField "m";
+                             csrFieldReserved "reserved" 36;
+                             @csrFieldAny "extensions" 26 None (* TODO *)
+                           ]%vector
+                    |}
+                  ]%vector
+           |};
+           {|
+             csrName := ^"mstatus";
+             csrAddr := CsrIdWidth 'h"300";
+             csrViews
+               := [
+                    {|
+                      csrViewContext := $1;
+                      csrViewNumFields := _;
+                      csrViewFields
+                        := [
+                             csrFieldReserved "reserved0" 19;
+                             @csrFieldAny "mpp" 2 None;
+                             csrFieldReserved "hpp" 2;
+                             @csrFieldAny "spp" 1 None;
+                             @csrFieldAny "mpie" 1 None;
+                             csrFieldReserved "hpie" 1;
+                             @csrFieldAny "spie" 1 None;
+                             @csrFieldAny "upie" 1 None;
+                             @csrFieldAny "mie" 1 None;
+                             csrFieldReserved "hie" 1;
+                             @csrFieldAny "sie" 1 None;
+                             @csrFieldAny "uie" 1 None
+                           ]%vector
+                    |};
+                    {|
+                      csrViewContext := $2;
+                      csrViewNumFields := _;
+                      csrViewFields
+                        := [
+                             csrFieldReserved "reserved0" 28;
+                             xlField "s";
+                             xlField "u";
+                             csrFieldReserved "reserved1" 19;
+                             @csrFieldAny "mpp" 2 None;
+                             csrFieldReserved "hpp" 2;
+                             @csrFieldAny "spp" 1 None;
+                             @csrFieldAny "mpie" 1 None;
+                             csrFieldReserved "hpie" 1;
+                             @csrFieldAny "spie" 1 None;
+                             @csrFieldAny "upie" 1 None;
+                             @csrFieldAny "mie" 1 None;
+                             csrFieldReserved "hie" 1;
+                             @csrFieldAny "sie" 1 None;
+                             @csrFieldAny "uie" 1 None
+                           ]%vector
+                    |}
+                  ]%vector
+           |};
+           {|
+             csrName := ^"mtvec";
+             csrAddr := CsrIdWidth 'h"305";
+             csrViews
+               := [
+                    {|
+                      csrViewContext := $1;
+                      csrViewNumFields := _;
+                      csrViewFields
+                        := [
+                             @csrFieldAny "mtvec_mode" 2 None;
+                             @csrFieldAny "mtvec_base" 30 None
+                           ]%vector
+                    |};
+                    {|
+                      csrViewContext := $2;
+                      csrViewNumFields := _;
+                      csrViewFields
+                        := [
+                             @csrFieldAny "mtvec_mode" 2 None;
+                             @csrFieldAny "mtvec_base" 62 None
+                           ]%vector
+                    |}
+                  ]%vector
+           |};
+           {|
+             csrName := ^"mscratch";
+             csrAddr := CsrIdWidth 'h"340";
+             csrViews
+               := [
+                    {|
+                      csrViewContext := $1;
+                      csrViewNumFields := _;
+                      csrViewFields
+                        := [
+                             @csrFieldAny "mscratch" 32 None
+                           ]%vector
+                    |};
+                    {|
+                      csrViewContext := $2;
+                      csrViewNumFields := _;
+                      csrViewFields
+                        := [
+                             @csrFieldAny "mscratch" 64 None
+                           ]%vector
+                    |}
+                  ]%vector
+           |};
+           {|
+             csrName := ^"mepc";
+             csrAddr := CsrIdWidth 'h"341";
+             csrViews
+               := [
+                    {|
+                      csrViewContext := $1;
+                      csrViewNumFields := _;
+                      csrViewFields
+                        := [
+                             @csrFieldAny "mepc" 32 None
+                           ]%vector
+                    |};
+                    {|
+                      csrViewContext := $2;
+                      csrViewNumFields := _;
+                      csrViewFields
+                        := [
+                             @csrFieldAny "mepc" 64 None
+                           ]%vector
+                    |}
+                  ]%vector
+           |};
+           {|
+             csrName := ^"mcause";
+             csrAddr := CsrIdWidth 'h"342";
+             csrViews
+               := [
+                    {|
+                      csrViewContext := $1;
+                      csrViewNumFields := _;
+                      csrViewFields
+                        := [
+                             @csrFieldAny "mcause_interrupt" 1 None;
+                             @csrFieldAny "mcause_code" 31 None
+                           ]%vector
+                    |};
+                    {|
+                      csrViewContext := $2;
+                      csrViewNumFields := _;
+                      csrViewFields
+                        := [
+                             @csrFieldAny "mcause_interrupt" 1 None;
+                             @csrFieldAny "mcause_code" 63 None
+                           ]%vector
+                    |}
+                  ]%vector
+           |};
+           {|
+             csrName := ^"mtval";
+             csrAddr := CsrIdWidth 'h"343";
+             csrViews
+               := [
+                    {|
+                      csrViewContext := $1;
+                      csrViewNumFields := _;
+                      csrViewFields
+                        := [
+                             @csrFieldAny "mtval" 32 None
+                           ]%vector
+                    |};
+                    {|
+                      csrViewContext := $2;
+                      csrViewNumFields := _;
+                      csrViewFields
+                        := [
+                             @csrFieldAny "mtval" 64 None
+                           ]%vector
+                    |}
+                  ]%vector
+           |};
+           {|
+             csrName := ^"sstatus";
+             csrAddr := CsrIdWidth 'h"100";
+             csrViews
+               := [
+                    {|
+                      csrViewContext := $1;
+                      csrViewNumFields := _;
+                      csrViewFields
+                        := [
+                             csrFieldReserved "reserved0" 23;
+                             @csrFieldAny "spp" 1 None;
+                             csrFieldReserved "reserved1" 2;
+                             @csrFieldAny "spie" 1 None;
+                             @csrFieldAny "upie" 1 None;
+                             csrFieldReserved "reserved2" 2;
+                             @csrFieldAny "sie" 1 None;
+                             @csrFieldAny "uie" 1 None
+                           ]%vector
+                    |};
+                    {|
+                      csrViewContext := $2;
+                      csrViewNumFields := _;
+                      csrViewFields
+                        := [
+                             csrFieldReserved "reserved0" 30;
+                             xlField "u";
+                             csrFieldReserved "reserved1" 23;
+                             @csrFieldAny "spp" 1 None;
+                             csrFieldReserved "reserved2" 2;
+                             @csrFieldAny "spie" 1 None;
+                             @csrFieldAny "upie" 1 None;
+                             csrFieldReserved "reserved3" 2;
+                             @csrFieldAny "sie" 1 None;
+                             @csrFieldAny "uie" 1 None
+                           ]%vector
+                    |}
+                  ]%vector
+           |};
+           {|
+             csrName := ^"stvec";
+             csrAddr := CsrIdWidth 'h"105";
+             csrViews
+               := [
+                    {|
+                      csrViewContext := $1;
+                      csrViewNumFields := _;
+                      csrViewFields
+                        := [
+                             @csrFieldAny "stvec_mode" 2 None;
+                             @csrFieldAny "stvec_base" 30 None
+                           ]%vector
+                    |};
+                    {|
+                      csrViewContext := $2;
+                      csrViewNumFields := _;
+                      csrViewFields
+                        := [
+                             @csrFieldAny "stvec_mode" 2 None;
+                             @csrFieldAny "stvec_base" 62 None
+                           ]%vector
+                    |}
+                  ]%vector
+           |};
+           {|
+             csrName := ^"sscratch";
+             csrAddr := CsrIdWidth 'h"140";
+             csrViews
+               := [
+                    {|
+                      csrViewContext := $1;
+                      csrViewNumFields := _;
+                      csrViewFields
+                        := [
+                             @csrFieldAny "sscratch" 32 None
+                           ]%vector
+                    |};
+                    {|
+                      csrViewContext := $2;
+                      csrViewNumFields := _;
+                      csrViewFields
+                        := [
+                             @csrFieldAny "sscratch" 64 None
+                           ]%vector
+                    |}
+                  ]%vector
+           |};
+           {|
+             csrName := ^"sepc";
+             csrAddr := CsrIdWidth 'h"141";
+             csrViews
+               := [
+                    {|
+                      csrViewContext := $1;
+                      csrViewNumFields := _;
+                      csrViewFields
+                        := [
+                             @csrFieldAny "sepc" 32 None
+                           ]%vector
+                    |};
+                    {|
+                      csrViewContext := $2;
+                      csrViewNumFields := _;
+                      csrViewFields
+                        := [
+                             @csrFieldAny "sepc" 64 None
+                           ]%vector
+                    |}
+                  ]%vector
+           |};
+           {|
+             csrName := ^"scause";
+             csrAddr := CsrIdWidth 'h"142";
+             csrViews
+               := [
+                    {|
+                      csrViewContext := $1;
+                      csrViewNumFields := _;
+                      csrViewFields
+                        := [
+                             @csrFieldAny "scause_interrupt" 1 None;
+                             @csrFieldAny "scause_code" 31 None
+                           ]%vector
+                    |};
+                    {|
+                      csrViewContext := $2;
+                      csrViewNumFields := _;
+                      csrViewFields
+                        := [
+                             @csrFieldAny "scause_interrupt" 1 None;
+                             @csrFieldAny "scause_code" 63 None
+                           ]%vector
+                    |}
+                  ]%vector
+           |};
+           {|
+             csrName := ^"stval";
+             csrAddr := CsrIdWidth 'h"143";
+             csrViews
+               := [
+                    {|
+                      csrViewContext := $1;
+                      csrViewNumFields := _;
+                      csrViewFields
+                        := [
+                             @csrFieldAny "stval" 32 None
+                           ]%vector
+                    |};
+                    {|
+                      csrViewContext := $2;
+                      csrViewNumFields := _;
+                      csrViewFields
+                        := [
+                             @csrFieldAny "stval" 64 None
+                           ]%vector
+                    |}
+                  ]%vector
+           |}
+         ].
+
+    Definition readCSR
+      (cfg_pkt : ContextCfgPkt @# ty)
+      (context_pkt : CSRWriteState @# ty)
+      (csrId : CsrId @# ty)
+      :  ActionT ty CsrValue
+      := LETA result
+           :  Maybe CsrValue
+           <- csrReadWrite CSRs cfg_pkt context_pkt
+                (STRUCT {
+                   "isRd"        ::= $$true;
+                   "addr"        ::= csrId;
+                   "contextCode" ::= cfg_pkt @% "xlen";
+                   "data"        ::= ($0 : CsrValue @# ty)
+                 } : LocationReadWriteInputT CsrValue @# ty);
+         Ret (#result @% "data").
+
+    Definition writeCSR
+      (cfg_pkt : ContextCfgPkt @# ty)
+      (context_pkt : CSRWriteState @# ty)
+      (csrId : CsrId @# ty)
+      (raw_data : Data @# ty)
+      :  ActionT ty Void
+      := LETA result
+           :  Maybe CsrValue
+           <- csrReadWrite CSRs cfg_pkt context_pkt
+                (STRUCT {
+                   "isRd"        ::= $$false;
+                   "addr"        ::= csrId;
+                   "contextCode" ::= cfg_pkt @% "xlen";
+                   "data"        ::= ZeroExtendTruncLsb CsrValueWidth raw_data
+                 } : LocationReadWriteInputT CsrValue @# ty);
+         Retv.
+
+    Close Scope kami_action.
+(*
+    Record CSR
+      := {
+           csrName : string;
+           csrAddr : word CsrIdWidth;
+           csrFields : Vector.t CSRField 2
+         }.
+
+    Definition csrReadWrite
+      (k : Kind)
+      (req : LocationReadWriteInputT k @# ty)
+      (entries : list CSR)
+      :  ActionT ty (Maybe k)
+      := utila_acts_find_pkt
+           (map
+             (fun csr_entry : CSR
+               => utila_acts_find_pkt
+                    (map
+                      (fun field_entry : CSRField
+                        => LET entry_match
+                             :  Bool
+                             <- ((req @% "addr") == $$(csrAddr csr_entry) &&
+                                 (req @% "contextCode") == csr
 
     Definition CSREntries
       :  list Location 
@@ -814,10 +1640,10 @@ Section Params.
            DispString _ "\n"
          ];
          Retv.
-
     Close Scope kami_expr.
 
     Close Scope kami_action.
+*)
 
   End CsrInterface.
 
@@ -1428,22 +2254,24 @@ Section Params.
       (reg_id : RegId @# ty)
       :  ActionT ty Data
       := Call reg_val
-           :  Array 1 Data
+           :  Data
            <- (^"read_reg_" ++ natToHexStr n) (reg_id : RegId);
-           Ret (IF reg_id == $0 then $0 else xlen_sign_extend Rlen xlen (ReadArrayConst #reg_val Fin.F1)).
+           Ret (xlen_sign_extend Rlen xlen #reg_val).
 
     Definition reg_reader_read_freg n
                (freg_id : RegId @# ty)
       :  ActionT ty Data
       := Call freg_val
-           :  Array 1 (Bit Flen)
+           :  Bit Flen
            <- (^"read_freg_" ++ natToHexStr n) (freg_id : RegId);
-           Ret (flen_one_extend Rlen (ReadArrayConst #freg_val Fin.F1)).
+           Ret (flen_one_extend Rlen (#freg_val)).
     
     Import ListNotations.
 
     Definition reg_reader_read_csr
-      (xlen : XlenValue @# ty)
+      (* (xlen : XlenValue @# ty) *)
+      (cfg_pkt : ContextCfgPkt @# ty)
+      (context_pkt : CSRWriteState @# ty)
       (raw_instr : Inst @# ty)
       :  ActionT ty (Maybe CsrValue)
       (*
@@ -1459,7 +2287,7 @@ Section Params.
       *)
       := LETA csr_value
            :  CsrValue
-           <- readCSR xlen (imm raw_instr);
+           <- readCSR cfg_pkt context_pkt (imm raw_instr);
          System [
            DispString _ "Read CSR Register\n";
            DispString _ "  CSR ID: ";
@@ -1472,20 +2300,27 @@ Section Params.
          Ret (Valid (#csr_value) : Maybe CsrValue @# ty).
 
     Definition reg_reader
-      (xlen : XlenValue @# ty)
+      (* (xlen : XlenValue @# ty) *)
+      (cfg_pkt : ContextCfgPkt @# ty)
       (decoder_pkt : DecoderPkt @# ty)
       :  ActionT ty ExecContextPkt
       := LET raw_inst
            :  Inst
            <- decoder_pkt @% "inst";
-         LETA reg1_val  : Data <- reg_reader_read_reg  1 xlen (rs1 #raw_inst);
-         LETA reg2_val  : Data <- reg_reader_read_reg  2 xlen (rs2 #raw_inst);
+         LETA reg1_val  : Data <- reg_reader_read_reg  1 (cfg_pkt @% "xlen") (rs1 #raw_inst);
+         LETA reg2_val  : Data <- reg_reader_read_reg  2 (cfg_pkt @% "xlen") (rs2 #raw_inst);
          LETA freg1_val : Data <- reg_reader_read_freg 1 (rs1 #raw_inst);
          LETA freg2_val : Data <- reg_reader_read_freg 2 (rs2 #raw_inst);
          LETA freg3_val : Data <- reg_reader_read_freg 3 (rs3 #raw_inst);
          LETA csr_val
            :  Maybe CsrValue
-           <- reg_reader_read_csr xlen #raw_inst;
+           (* <- reg_reader_read_csr xlen #raw_inst; *)
+           <- reg_reader_read_csr cfg_pkt
+                (STRUCT {
+                   "pc"          ::= decoder_pkt @% "pc";
+                   "compressed?" ::= decoder_pkt @% "compressed?"
+                 } : CSRWriteState @# ty)
+                #raw_inst;
          Read fflags_val : FflagsValue <- ^"fflags";
          Read frm_val : FrmValue <- ^"frm";
          LETA msg <- Sys [
@@ -1540,12 +2375,14 @@ Section Params.
               } : ExecContextPkt @# ty).
 
     Definition readerWithException
-      (xlen : XlenValue @# ty)
+      (* (xlen : XlenValue @# ty) *)
+      (cfg_pkt : ContextCfgPkt @# ty)
       (decoder_pkt : PktWithException DecoderPkt @# ty)
       :  ActionT ty (PktWithException ExecContextPkt)
       := LETA exec_context_pkt
            <- reg_reader
-                xlen
+                (* xlen *)
+                cfg_pkt
                 ((decoder_pkt @% "fst") : DecoderPkt @# ty);
          Ret
            (mkPktWithException
@@ -1596,8 +2433,8 @@ Section Params.
         := LET pkt
              :  IntRegWrite
              <- STRUCT {
-                  "addr" ::= reg_id;
-                  "data"  ::= ARRAY { xlen_sign_extend Xlen xlen data }
+                  "index" ::= reg_id;
+                  "data"  ::= xlen_sign_extend Xlen xlen data
                 };
            Call ^"regWrite" (#pkt : IntRegWrite);
            System [
@@ -1616,8 +2453,8 @@ Section Params.
         := LET pkt
              :  FloatRegWrite
              <- STRUCT {
-                  "addr" ::= reg_id;
-                  "data"  ::= ARRAY { OneExtendTruncLsb Flen data }
+                  "index" ::= reg_id;
+                  "data"  ::= OneExtendTruncLsb Flen data
                 };
            Call (^"fregWrite") (#pkt : FloatRegWrite);
            System [
@@ -1720,7 +2557,9 @@ Section Params.
              Retv.
 
       Definition commitWriters
-        (xlen : XlenValue @# ty)
+        (* (xlen : XlenValue @# ty) *)
+        (cfg_pkt : ContextCfgPkt @# ty)
+        (context_pkt : CSRWriteState @# ty)
         (val: Maybe RoutedReg @# ty)
         (reg_index: RegId @# ty)
         (csr_index: CsrId @# ty)
@@ -1731,13 +2570,15 @@ Section Params.
              then 
                (If (#val_pos == $IntRegTag)
                   then (If (reg_index != $0)
-                          then reg_writer_write_reg xlen (reg_index) (#val_data);
+                          (* then reg_writer_write_reg xlen (reg_index) (#val_data); *)
+                          then reg_writer_write_reg (cfg_pkt @% "xlen") (reg_index) (#val_data);
                         Retv)
                   else (If (#val_pos == $FloatRegTag)
                           then reg_writer_write_freg (reg_index) (#val_data)
                           else (If (#val_pos == $CsrTag)
                                   then
-                                    (LETA _ <- writeCSR xlen csr_index (#val_data);
+                                    (* (LETA _ <- writeCSR xlen csr_index (#val_data); *)
+                                    (LETA _ <- writeCSR cfg_pkt context_pkt csr_index (#val_data);
                                      System [
                                        DispString _ "  [commitWriters] wrote to CSR.\n";
                                        DispString _ "  [commitWriters] value data: ";
@@ -1762,7 +2603,7 @@ Section Params.
                                           else
                                             (If (#val_pos == $RetTag)
                                                then
-                                                 (LETA _ <- commitRet val;
+                                                 ((* LETA _ <- commitRet val; *) (* TODO uncomment once registers ported over. *)
                                                   System [
                                                     DispString _ "Executing Ret Instruction.\n"
                                                   ];
@@ -1816,8 +2657,18 @@ Section Params.
                  Retv
              else (
 *)
+(*
                 LETA _ <- commitWriters (cfg_pkt @% "xlen") #val1 #reg_index #csr_index;
                 LETA _ <- commitWriters (cfg_pkt @% "xlen") #val2 #reg_index #csr_index; 
+*)
+                LET context_pkt
+                  :  CSRWriteState
+                  <- STRUCT {
+                       "pc" ::= pc;
+                       "compressed?" ::= exec_context_pkt @% "compressed?"
+                     }; 
+                LETA _ <- commitWriters cfg_pkt #context_pkt #val1 #reg_index #csr_index;
+                LETA _ <- commitWriters cfg_pkt #context_pkt #val2 #reg_index #csr_index; 
                 LET opt_val1 <- cxt @% "fst" @% "val1";
                 LET opt_val2 <- cxt @% "fst" @% "val2";
                 Read mepc : VAddr <- ^"mepc";
